EIP20 changes

execution/examples/EIP20Token.v
@@ -1,11 +1,11 @@
 (*
   This file contains an implementation of the EIP 20 Token Specification (https://eips.ethereum.org/EIPS/eip-20).
   The implementation is essentially a port of https://github.com/ConsenSys/Tokens/blob/fdf687c69d998266a95f15216b1955a4965a0a6d/contracts/eip20/EIP20.sol
-
 *)
-
 From Coq Require Import ZArith.
 From Coq Require Import List.
+From ConCert.Execution Require Import Automation.
+From ConCert.Execution Require Import Containers.
 From ConCert.Execution Require Import Monads.
 From ConCert.Execution Require Import Extras.
 From ConCert.Execution Require Import Serializable.
@@ -38,8 +38,8 @@ Section EIP20Token.
 
   Record Setup :=
     build_setup {
-  owner : Address;
-  init_amount : TokenValue;
+      owner : Address;
+      init_amount : TokenValue;
     }.
 
   MetaCoq Run (make_setters State).
@@ -85,7 +85,6 @@ Section EIP20Token.
 
 (* The delegate tries to transfer <amount> tokens from <from> to <to>.
    Succeeds if <from> has indeed allowed the delegate to spend at least <amount> tokens on its behalf. *)
-
   Definition try_transfer_from (delegate : Address)
        (from : Address)
        (to : Address)
@@ -136,4 +135,684 @@ Section EIP20Token.
   Definition contract : Contract Setup Msg State :=
     build_contract init receive.
 
+
+
+Section Theories.
+
+Import Lia.
+Import Permutation.
+
+(* ------------------- EIP20 functions not payable ------------------- *)
+
+(* receive only returns Some if the sender amount is zero *)
+Lemma EIP20_not_payable : forall prev_state new_state chain ctx msg new_acts,
+  receive chain ctx prev_state msg = Some (new_state, new_acts) ->
+    ((ctx_amount ctx) <= 0)%Z.
+Proof.
+  intros * receive_some.
+  unfold receive in receive_some.
+  destruct_match eqn:amount in receive_some.
+  - (* case: ctx_amount > 0 *)
+    congruence.
+  - (* case: ctx_amount <= 0 *)
+    now rewrite Z.gtb_ltb, Z.ltb_ge in amount.
+Qed.
+
+(* Lemma for simplifying the receive function by eliminating the case
+    where sender amount is larger than zero *)
+Lemma receive_not_payable : forall prev_state new_state chain ctx msg new_acts,
+  receive chain ctx prev_state (Some msg) = Some (new_state, new_acts) ->
+    match msg with
+    | transfer to amount => option_map (fun new_state : State => (new_state, [])) (try_transfer (ctx_from ctx) to amount prev_state)
+    | transfer_from from to amount =>
+        option_map (fun new_state : State => (new_state, [])) (try_transfer_from (ctx_from ctx) from to amount prev_state)
+    | approve delegate amount =>
+        option_map (fun new_state : State => (new_state, [])) (try_approve (ctx_from ctx) delegate amount prev_state)
+    end = Some (new_state, new_acts).
+Proof.
+  intros * receive_some.
+  apply EIP20_not_payable in receive_some as amount_zero.
+  unfold receive in receive_some.
+  rewrite <- Z.ltb_ge, <- Z.gtb_ltb in amount_zero.
+  now rewrite amount_zero in receive_some.
+Qed.
+
+
+
+(* ------------------- EIP20 functions produce no acts ------------------- *)
+
+(* receive never produces any new_acts *)
+Lemma EIP20_no_acts : forall prev_state new_state chain ctx msg new_acts,
+  receive chain ctx prev_state msg = Some (new_state, new_acts) ->
+    new_acts = [].
+Proof.
+  intros * receive_some.
+  unfold receive, option_map in receive_some.
+  repeat destruct_match in receive_some; try congruence.
+Qed.
+
+Lemma receive_no_acts : forall prev_state new_state chain ctx msg new_acts,
+  receive chain ctx prev_state (Some msg) = Some (new_state, new_acts) ->
+    receive chain ctx prev_state (Some msg) = Some (new_state, []).
+Proof.
+  intros.
+  now erewrite <- EIP20_no_acts.
+Qed.
+
+
+
+(* ------------------- Default entrypoint always fail ------------------- *)
+
+Lemma default_none : forall prev_state chain ctx,
+  receive chain ctx prev_state None = None.
+Proof.
+  intros.
+  unfold receive.
+  now destruct_match.
+Qed.
+
+
+
+(* ------------------- FMap partial alter is FMap add ------------------- *)
+
+Lemma add_is_partial_alter_plus : forall (account : Address) amount (balances : FMap Address N) (f : N -> N),
+  FMap.partial_alter (fun balance : option N => Some (with_default 0 balance + amount)) account balances =
+  FMap.add account (with_default 0 (FMap.find account balances) + amount) balances.
+Proof.
+  intros.
+  now apply fin_maps.partial_alter_ext.
+Qed.
+
+Lemma increment_balanace_is_partial_alter_plus : forall (addr : Address) amount (m : FMap Address N),
+  increment_balance m addr amount =
+  FMap.partial_alter (fun balance : option N => Some (with_default 0 balance + amount)) addr m.
+Proof.
+  intros.
+  unfold increment_balance, AddressMap.add, AddressMap.find.
+  rewrite add_is_partial_alter_plus by auto.
+  destruct_match eqn:addr_in_map;
+    now setoid_rewrite addr_in_map.
+Qed.
+
+
+
+(* ------------------- Tactic to simplify proof steps ------------------- *)
+
+Ltac receive_simpl_step :=
+  match goal with
+  | H : receive _ _ _ (Some _) = Some (_, _) |- _ =>
+    apply receive_no_acts, receive_not_payable in H; cbn in H
+  | |- receive _ _ _ (Some _) = Some (_, _) =>
+    apply receive_no_acts, receive_not_payable; cbn
+  | H : context[receive] |- _ => unfold receive in H
+  | |- context[receive] => unfold receive
+  | H : context[Blockchain.receive] |- _ => unfold Blockchain.receive; cbn in H
+  | H : context[try_transfer] |- _ => unfold try_transfer in H
+  | H : context[try_transfer_from] |- _ => unfold try_transfer_from in H
+  | H : context[try_approve] |- _ => unfold try_approve in H
+  | |- context[Blockchain.receive] => unfold Blockchain.receive; cbn
+  | |- context[try_transfer] => unfold try_transfer
+  | |- context[try_transfer_from] => unfold try_transfer_from
+  | |- context[try_approve] => unfold try_approve
+  | H : context [ AddressMap.find _ _ ] |- _ => rewrite AddressMap_find_convertible in H
+  | H : context [ AddressMap.add _ _ _ ] |- _ =>  rewrite AddressMap_add_convertible in H
+  | H : context [ increment_balance _ _ _ ] |- _ => rewrite increment_balanace_is_partial_alter_plus in H
+  | |- context [ AddressMap.find _ _ ] => rewrite AddressMap_find_convertible
+  | |- context [ AddressMap.add _ _ _ ] => rewrite AddressMap_add_convertible
+  | |- context [ increment_balance _ _ _ ] => rewrite increment_balanace_is_partial_alter_plus
+  | H : option_map (fun s : State => (s, _)) match ?m with | Some _ => _ | None => None end = Some _ |- _ =>
+    let a := fresh "H" in
+    destruct m eqn:a in H; try setoid_rewrite a; cbn in *; try congruence
+  | H : option_map (fun s : State => (s, _)) (if ?m then ?a else ?b) = Some _ |- _ =>
+    match a with
+    | None =>
+      let a := fresh "H" in
+      destruct m eqn:a in H; try setoid_rewrite a; cbn in *; try congruence
+    | _ => match b with
+           | None =>
+             let a := fresh "H" in
+             destruct m eqn:a in H; try setoid_rewrite a; cbn in *; try congruence
+           | _ => idtac
+    end end
+  | H : (if ?m then ?a else ?b) = Some _ |- _ =>
+    match a with
+    | None =>
+      let a := fresh "H" in
+      destruct m eqn:a in H; try setoid_rewrite a; cbn in *; try congruence
+    | _ => match b with
+           | None =>
+             let a := fresh "H" in
+             destruct m eqn:a in H; try setoid_rewrite a; cbn in *; try congruence
+           | _ => idtac
+    end end
+  end.
+
+Tactic Notation "receive_simpl" := repeat receive_simpl_step.
+
+Ltac FMap_simpl_step :=
+  match goal with
+    | |- context [ FMap.find ?x (FMap.add ?x _ _) ] => setoid_rewrite FMap.find_add
+    | H : FMap.find ?t ?m = Some _ |- FMap.find ?t ?m = Some _ => cbn; rewrite H; f_equal; lia
+    | H : ?x <> ?y |- context [ FMap.find ?x (FMap.add ?y _ _) ] => setoid_rewrite FMap.find_add_ne; eauto
+    | H : ?y <> ?x |- context [ FMap.find ?x (FMap.add ?y _ _) ] => setoid_rewrite FMap.find_add_ne; eauto
+    | H : FMap.find ?x _ = Some _ |- context [ FMap.elements (FMap.add ?x _ _) ] => setoid_rewrite FMap.elements_add_existing; eauto
+    | |- context [ FMap.add ?x _ (FMap.add ?x _ _) ] => setoid_rewrite FMap.add_add
+    | H : FMap.find ?x _ = None |- context [ FMap.elements (FMap.add ?x _ _) ] => setoid_rewrite FMap.elements_add; eauto
+    | |- context [ FMap.remove ?x (FMap.add ?x _ _) ] => rewrite fin_maps.delete_insert_delete
+    | |- context [ FMap.find ?x (FMap.partial_alter _ ?x _) ] => setoid_rewrite FMap.find_partial_alter
+    | H : ?x' <> ?x |- context [ FMap.find ?x' (FMap.partial_alter _ ?x _) ] => setoid_rewrite FMap.find_partial_alter_ne; auto
+    | H : ?x <> ?x' |- context [ FMap.find ?x' (FMap.partial_alter _ ?x _) ] => setoid_rewrite FMap.find_partial_alter_ne
+    | H : context [ AddressMap.find _ _ ] |- _ => rewrite AddressMap_find_convertible in H
+    | H : context [ AddressMap.add _ _ _ ] |- _ =>  rewrite AddressMap_add_convertible in H
+    | H : context [ increment_balance _ _ _ ] |- _ => rewrite increment_balanace_is_partial_alter_plus in H
+    | |- context [ AddressMap.find _ _ ] => rewrite AddressMap_find_convertible
+    | |- context [ AddressMap.add _ _ _ ] =>  rewrite AddressMap_add_convertible
+    | |- context [ increment_balance _ _ _ ] => rewrite increment_balanace_is_partial_alter_plus
+   end.
+
+Tactic Notation "FMap_simpl" := repeat (FMap_simpl_step; cbn).
+
+
+
+(* ------------------- isSome function ------------------- *)
+
+Definition isSome {A : Type} (a : option A) := match a with | Some _ => true | None => false end.
+
+(* if x is None then with_default is equal to default element *)
+Lemma with_default_is_some : forall {A : Type} (x : option A) (y : A),
+  isSome x = false ->
+    with_default y x = y.
+Proof.
+  now destruct x.
+Qed.
+
+
+
+(* ------------------- sumN function ------------------- *)
+
+(* sumN of balances is the same after transfer changes if sender has enough balance *)
+Lemma sumN_FMap_add_sub : forall from to amount (balances : FMap Address N),
+  amount <= with_default 0 (FMap.find from balances) ->
+    (sumN (fun '(_, v) => v) (FMap.elements balances)) =
+    (sumN(fun '(_, v) => v)
+       (FMap.elements
+          (FMap.partial_alter (fun balance : option N => Some (with_default 0 balance + amount)) to
+             (FMap.add from (with_default 0 (FMap.find from balances) - amount) balances)))).
+Proof.
+  intros from to amount balances from_enough_balance.
+  rewrite add_is_partial_alter_plus; auto.
+  edestruct (address_eqb from to) eqn:from_to_eq;
+    destruct FMap.find eqn:from_prev;
+    destruct_address_eq; try discriminate; subst; cbn in *;
+    repeat match goal with
+    | H : _ <= 0 |- _ => apply N.lt_eq_cases in H as [H | H]; try lia; subst
+    | |- context [ with_default _ (FMap.find to balances) ] => destruct (FMap.find to balances) eqn:to_prev; cbn
+    | |- context [ FMap.find ?x (FMap.add ?x _ _) ] => rewrite FMap.find_add
+    | H : FMap.find ?t ?m = Some _ |- FMap.find ?t ?m = Some _ => cbn; rewrite H; f_equal; lia
+    | H : ?x <> ?y |- context [ FMap.find ?x (FMap.add ?y _ _) ] => rewrite FMap.find_add_ne; eauto
+    | H : ?y <> ?x |- context [ FMap.find ?x (FMap.add ?y _ _) ] => rewrite FMap.find_add_ne; eauto
+    | H : FMap.find ?x _ = Some _ |- context [ FMap.elements (FMap.add ?x _ _) ] => rewrite FMap.elements_add_existing; eauto
+    | |- context [ FMap.add ?x _ (FMap.add ?x _ _) ] => rewrite FMap.add_add
+    | H : FMap.find ?x _ = None |- context [ FMap.elements (FMap.add ?x _ _) ] => rewrite FMap.elements_add; eauto
+    | |- context [ FMap.remove ?x (FMap.add ?x _ _) ] => rewrite fin_maps.delete_insert_delete
+    | H : FMap.find ?x ?m = Some _ |- context [ sumN _ ((_, _) :: FMap.elements (FMap.remove ?x ?m)) ] => rewrite fin_maps.map_to_list_delete; auto
+    | H : FMap.find ?x _ = Some ?n |- context [ sumN _ ((?x, ?n) :: FMap.elements (FMap.remove ?x _)) ] => rewrite fin_maps.map_to_list_delete; auto
+    | H : FMap.find ?x _ = Some ?n |- context [ sumN _ ((?x, ?n) :: (_, _) :: FMap.elements (FMap.remove ?x _)) ] => rewrite sumN_swap, fin_maps.map_to_list_delete; auto
+    | |- context [ _ + 0 ] => rewrite N.add_0_r
+    | |- context [ 0 + _ ] => rewrite N.add_0_l
+    | |- context [ sumN _ ((?t, ?n + ?m) :: _) ] => erewrite sumN_split with (x:= (t, n)) (y := (_, m)) by lia
+    | |- context [ sumN _ ((_, ?n) :: (_, ?m - ?n) :: _) ] => erewrite <- sumN_split with (z := (_, n + m - n)) by lia
+   end.
+   Unshelve. eauto.
+Qed.
+
+(* sum of all balances in the token state *)
+Definition sum_balances (state : EIP20Token.State) :=
+  sumN (fun '(k, v) => v) (FMap.elements (balances state)).
+
+
+
+(* ------------------- Expected behvaiour of EIP20 functions ------------------- *)
+
+Definition transfer_balance_update_correct old_state new_state from to tokens :=
+  let get_balance addr state := with_default 0 (FMap.find addr state.(balances)) in
+  let from_balance_before := get_balance from old_state in
+  let to_balance_before := get_balance to old_state in
+  let from_balance_after := get_balance from new_state in
+  let to_balance_after := get_balance to new_state in
+  (* if the transfer is a self-transfer, balances should remain unchained *)
+  if address_eqb from to
+  then
+    (from_balance_before =? from_balance_after) &&
+    (to_balance_before =? to_balance_after)
+  else
+    (from_balance_before =? from_balance_after + tokens) &&
+    (to_balance_before + tokens =? to_balance_after).
+
+Definition get_allowance state from delegate :=
+  with_default 0 (FMap.find delegate (with_default (@FMap.empty (FMap Address TokenValue) _) (FMap.find from (allowances state)))).
+
+Definition transfer_from_allowances_update_correct (old_state new_state : State) (from delegate : Address) (tokens : TokenValue) :=
+  let delegate_allowance_before := get_allowance old_state from delegate in
+  let delegate_allowance_after := get_allowance new_state from delegate in 
+    delegate_allowance_before =? delegate_allowance_after + tokens.
+
+Definition approve_allowance_update_correct (new_state : State) (from delegate : Address) (tokens : TokenValue) :=
+  let delegate_allowance_after := get_allowance new_state from delegate in
+    delegate_allowance_after =? tokens.
+
+
+
+(* ------------------- Transfer correct ------------------- *)
+
+(* try_transfer correctly moves <amount> from <sender> to <to> *)
+Lemma try_transfer_balance_correct : forall prev_state new_state chain ctx to amount new_acts,
+  receive chain ctx prev_state (Some (transfer to amount)) = Some (new_state, new_acts) ->
+  transfer_balance_update_correct prev_state new_state ctx.(ctx_from) to amount = true.
+Proof.
+  intros * receive_some.
+  unfold transfer_balance_update_correct.
+  receive_simpl.
+  rename H into sender_enough_balance.
+  apply N.ltb_ge in sender_enough_balance.
+  destruct_address_eq; destruct (FMap.find (ctx_from ctx) (balances prev_state)) eqn:from_prev;
+    try congruence; subst; try rewrite from_prev; inversion receive_some;
+    clear receive_some H0 from_prev new_acts chain; cbn in *.
+    - (* case: from =  to && find from = Some n && amount <= n *)
+      FMap_simpl.
+      now rewrite N.sub_add, N.eqb_refl.
+    - (* case: from =  to && find from = None   && amount = 0 *)
+      apply N.lt_eq_cases in sender_enough_balance as []; [lia | subst].
+      now FMap_simpl.
+    - (* case: from <> to && find from = Some n && amount <= n *)
+      FMap_simpl.
+      rewrite N.sub_add; auto.
+      now rewrite !N.eqb_refl.
+    - (* case: from <> to && find from = None   && amount = 0 *)
+      apply N.lt_eq_cases in sender_enough_balance as []; [lia | subst].
+      FMap_simpl.
+      apply N.eqb_refl.
+Qed.
+
+(* try_transfer does not change the total supply of tokens *)
+Lemma try_transfer_preserves_total_supply : forall prev_state new_state chain ctx to amount new_acts,
+  receive chain ctx prev_state (Some (transfer to amount)) = Some (new_state, new_acts) ->
+    (total_supply prev_state) = (total_supply new_state).
+Proof.
+  intros * receive_some.
+  receive_simpl.
+  now inversion receive_some.
+Qed.
+
+(* try_transfer does not change allowances *)
+Lemma try_transfer_preserves_allowances : forall prev_state new_state chain ctx to amount new_acts,
+  receive chain ctx prev_state (Some (transfer to amount)) = Some (new_state, new_acts) ->
+    (allowances prev_state) = (allowances new_state).
+Proof.
+  intros * receive_some.
+  receive_simpl.
+  now inversion receive_some.
+Qed.
+
+(* try_transfer only modifies the <sender> and <to> balances *)
+Lemma try_transfer_preserves_other_balances : forall prev_state new_state chain ctx to amount new_acts,
+  receive chain ctx prev_state (Some (transfer to amount)) = Some (new_state, new_acts) ->
+    forall account, account <> (ctx_from ctx) -> account <> to ->
+      FMap.find account (balances prev_state) = FMap.find account (balances new_state).
+Proof.
+  intros * receive_some account account_not_sender account_not_receiver.
+  receive_simpl.
+  inversion receive_some.
+  cbn.
+  FMap_simpl.
+Qed.
+
+(* If the requirements are met then then receive on transfer msg must succeed and
+    if receive on transfer msg succeeds then requirements must hold *)
+Lemma try_transfer_is_some : forall state chain ctx to amount,
+  (ctx_amount ctx >? 0)%Z = false ->
+  (amount = 0 /\ isSome (FMap.find (ctx_from ctx) (balances state)) = false)
+  \/ amount <= with_default 0 (FMap.find (ctx_from ctx) (balances state))
+    <-> isSome (receive chain ctx state (Some (transfer to amount))) = true.
+Proof.
+  intros * amount_positive.
+  split.
+  - intros [(amount_zero & sender_balance_some) | sender_enough_balance];
+    receive_simpl; destruct_match eqn:amount_from; auto.
+    + subst.
+      now erewrite with_default_is_some, N.ltb_irrefl by assumption.
+    + rewrite <- N.ltb_ge in sender_enough_balance.
+      now setoid_rewrite sender_enough_balance.
+  - intros receive_some. receive_simpl. rewrite amount_positive in receive_some.
+    destruct_match eqn:amount_from in receive_some.
+    + discriminate.
+    + now apply N.ltb_ge in amount_from.
+Qed.
+
+
+
+(* ------------------- Transfer_from correct ------------------- *)
+
+(* try_transfer_from correctly updates balance and allowance *)
+Lemma try_transfer_from_balance_correct : forall prev_state new_state chain ctx from to amount new_acts,
+  receive chain ctx prev_state (Some (transfer_from from to amount)) = Some (new_state, new_acts) ->
+  transfer_balance_update_correct prev_state new_state from to amount = true /\
+  transfer_from_allowances_update_correct prev_state new_state from ctx.(ctx_from) amount = true.
+Proof.
+  intros * receive_some.
+  unfold transfer_balance_update_correct,
+    transfer_from_allowances_update_correct,
+    get_allowance.
+  receive_simpl.
+  rename H into from_allowances.
+  rename H0 into sender_alloance.
+  apply Bool.orb_false_iff in H1 as (sender_enough_allowance%N.ltb_ge &
+                                     from_enough_balance%N.ltb_ge).
+  split.
+    + (* proof of balance updated correct *)
+    destruct_address_eq;
+      destruct (FMap.find from (balances prev_state)) eqn:from_bal_prev;
+      subst; try rewrite from_bal_prev; inversion receive_some;
+      cbn in *; clear receive_some H0.
+      * (* case: from =  to && find from = Some n && amount <= n *)
+        FMap_simpl.
+        now rewrite N.sub_add, N.eqb_refl.
+      * (* case: from =  to && find from = None   && amount = 0 *)
+        apply N.lt_eq_cases in from_enough_balance as []; [lia | subst].
+        now FMap_simpl.
+      * (* case: from <> to && find from = Some n && amount <= n *)
+        FMap_simpl.
+        rewrite N.sub_add by auto.
+        now rewrite ?N.eqb_refl.
+      * (* case: from <> to && find from = None   && amount = 0 *)
+        apply N.lt_eq_cases in from_enough_balance as []; [lia | subst].
+        FMap_simpl.
+        apply N.eqb_refl.
+    + (* proof of allowances updated correct *)
+      inversion receive_some.
+      cbn. FMap_simpl.
+      rewrite N.sub_add by auto.
+      apply N.eqb_refl.
+Qed.
+
+(* try_transfer_from does not change total supply of tokens *)
+Lemma try_transfer_from_preserves_total_supply : forall prev_state new_state chain ctx from to amount new_acts,
+  receive chain ctx prev_state (Some (transfer_from from to amount)) = Some (new_state, new_acts) ->
+    (total_supply prev_state) = (total_supply new_state).
+Proof.
+  intros * receive_some.
+  receive_simpl.
+  now inversion receive_some.
+Qed.
+
+(* try_transfer_from only changes <from> and <to> balances *)
+Lemma try_transfer_from_preserves_other_balances : forall prev_state new_state chain ctx from to amount new_acts,
+  receive chain ctx prev_state (Some (transfer_from from to amount)) = Some (new_state, new_acts) ->
+    forall account, account <> from -> account <> to ->
+      FMap.find account (balances prev_state) = FMap.find account (balances new_state).
+Proof.
+  intros * receive_some account account_not_from account_not_to.
+  receive_simpl.
+  inversion receive_some.
+  cbn.
+  FMap_simpl.
+Qed.
+
+(* try_transfer_from only changes allowance map of <from> *)
+Lemma try_transfer_from_preserves_other_allowances : forall prev_state new_state chain ctx from to amount new_acts,
+  receive chain ctx prev_state (Some (transfer_from from to amount)) = Some (new_state, new_acts) ->
+    forall account, account <> from ->
+      FMap.find account (allowances prev_state) = FMap.find account (allowances new_state).
+Proof.
+  intros * receive_some account account_not_from.
+  receive_simpl.
+  inversion receive_some.
+  cbn.
+  FMap_simpl.
+Qed.
+
+(* try_transfer_from only changes allowance of <sender> *)
+Lemma try_transfer_from_preserves_other_allowance : forall prev_state new_state chain ctx from to amount new_acts,
+  receive chain ctx prev_state (Some (transfer_from from to amount)) = Some (new_state, new_acts) ->
+    forall account, account <> (ctx_from ctx) ->
+      get_allowance prev_state from account = get_allowance new_state from account.
+Proof.
+  intros * receive_some account account_not_sender.
+  unfold get_allowance.
+  receive_simpl.
+  inversion receive_some.
+  cbn.
+  FMap_simpl.
+Qed.
+
+(* If the requirements are met then then receive on transfer_from msg must succeed and
+    if receive on transfer_from msg succeeds then requirements must hold *)
+Lemma try_transfer_from_is_some : forall state chain ctx from to amount,
+  let get_allowance_ account := FMap.find account (with_default (@FMap.empty (FMap Address TokenValue) _) (FMap.find from (allowances state))) in
+  (ctx_amount ctx >? 0)%Z = false ->
+  isSome (FMap.find from (allowances state)) = true
+  /\ isSome (get_allowance_ (ctx_from ctx)) = true
+  /\ amount <= with_default 0 (FMap.find from (balances state))
+  /\ amount <= with_default 0 (get_allowance_ (ctx_from ctx))
+    <-> isSome (receive chain ctx state (Some (transfer_from from to amount))) = true.
+Proof.
+  intros * sender_amount_zero.
+  split; receive_simpl; rewrite sender_amount_zero in *;
+    unfold get_allowance_; clear get_allowance_; cbn.
+  - intros (from_allowances_some &
+            sender_allowance &
+            from_enough_balance%N.ltb_ge &
+            sender_enough_allowance%N.ltb_ge).
+    destruct_match eqn:allowances_ctx; setoid_rewrite allowances_ctx in sender_allowance; auto.
+    setoid_rewrite allowances_ctx in sender_enough_allowance.
+    cbn in *. clear from_allowances_some.
+    destruct_match eqn:allowance_ctx; setoid_rewrite allowance_ctx in sender_allowance; auto.
+    setoid_rewrite allowance_ctx in sender_enough_allowance.
+    cbn in *. clear sender_allowance.
+    destruct_match eqn:amount_from; auto.
+    setoid_rewrite from_enough_balance in amount_from.
+    now setoid_rewrite sender_enough_allowance in amount_from.
+  - intros receive_some.
+    destruct_match eqn:allowances_ctx in receive_some; setoid_rewrite allowances_ctx; try discriminate.
+    destruct_match eqn:allowance_ctx in receive_some; setoid_rewrite allowance_ctx; try discriminate.
+    destruct_match eqn:amount_from in receive_some; try discriminate.
+    apply Bool.orb_false_iff in amount_from as
+      (from_enough_balance%N.ltb_ge & sender_enough_allowance%N.ltb_ge).
+    intuition.
+Qed.
+
+
+
+(* ------------------- Approve correct ------------------- *)
+
+(* try_approve correctly replaces allowance *)
+Lemma try_approve_allowance_correct : forall prev_state new_state chain ctx delegate amount new_acts,
+  receive chain ctx prev_state (Some (approve delegate amount)) = Some (new_state, new_acts) ->
+  approve_allowance_update_correct new_state ctx.(ctx_from) delegate amount = true.
+Proof.
+  intros * receive_some.
+  unfold approve_allowance_update_correct, get_allowance.
+  receive_simpl.
+  destruct_match eqn:from_allowance in receive_some;
+    inversion receive_some; cbn;
+    FMap_simpl; apply N.eqb_refl.
+Qed.
+
+(* try_approve does not change total supply of tokens *)
+Lemma try_approve_preserves_total_supply : forall prev_state new_state chain ctx delegate amount new_acts,
+  receive chain ctx prev_state (Some (approve delegate amount)) = Some (new_state, new_acts) ->
+    (total_supply prev_state) = (total_supply new_state).
+Proof.
+  intros * receive_some.
+  receive_simpl.
+  destruct_match in receive_some;
+    now inversion receive_some.
+Qed.
+
+(* try_approve does not change balances *)
+Lemma try_approve_preserves_balances : forall prev_state new_state chain ctx delegate amount new_acts,
+  receive chain ctx prev_state (Some (approve delegate amount)) = Some (new_state, new_acts) ->
+    (balances prev_state) = (balances new_state).
+Proof.
+  intros * receive_some.
+  receive_simpl.
+  destruct_match in receive_some;
+    now inversion receive_some.
+Qed.
+
+(* try_approve does not change allowances map of other addresses *)
+Lemma try_approve_preserves_other_allowances : forall prev_state new_state chain ctx delegate amount new_acts,
+  receive chain ctx prev_state (Some (approve delegate amount)) = Some (new_state, new_acts) ->
+    forall account, account <> (ctx_from ctx) ->
+      FMap.find account (allowances prev_state) = FMap.find account (allowances new_state).
+Proof.
+  intros * receive_some account account_not_sender.
+  receive_simpl.
+  destruct_match in receive_some;
+    inversion receive_some;
+    cbn; FMap_simpl.
+Qed.
+
+(* try_approve does not change allowance of other addresses *)
+Lemma try_approve_preserves_other_allowance : forall prev_state new_state chain ctx delegate amount new_acts,
+  receive chain ctx prev_state (Some (approve delegate amount)) = Some (new_state, new_acts) ->
+    forall account, account <> delegate ->
+      get_allowance prev_state (ctx_from ctx) account = get_allowance new_state (ctx_from ctx) account.
+Proof.
+  intros * receive_some account account_not_delegate.
+  receive_simpl.
+  unfold get_allowance.
+  destruct_match eqn:allowances_from in receive_some;
+    setoid_rewrite allowances_from;
+    inversion receive_some;
+    cbn; FMap_simpl.
+Qed.
+
+(* If the requirements are met then then receive on approve msg must succeed and
+    if receive on approve msg succeeds then requirements must hold *)
+Lemma try_approve_is_some : forall state chain ctx delegate amount,
+  (ctx_amount ctx >? 0)%Z = false <-> isSome (receive chain ctx state (Some (approve delegate amount))) = true.
+Proof.
+  split; receive_simpl.
+  - intros sender_amount_zero.
+    rewrite sender_amount_zero.
+    now destruct_match.
+  - intros receive_some.
+    now destruct_match in receive_some.
+Qed.
+
+
+
+(* ------------------- EIP20 functions preserve sum of balances ------------------- *)
+
+(* sum of all balances remain the same after proccessing transfer msg *)
+Lemma try_transfer_preserves_balances_sum : forall prev_state new_state chain ctx to amount new_acts,
+  receive chain ctx prev_state (Some (transfer to amount)) = Some (new_state, new_acts) ->
+    (sum_balances prev_state) = (sum_balances new_state).
+Proof.
+  intros * receive_some.
+  receive_simpl.
+  rename H into sender_enough_balance.
+  apply N.ltb_ge in sender_enough_balance.
+  inversion receive_some.
+  unfold sum_balances. cbn.
+  now apply sumN_FMap_add_sub.
+Qed.
+
+(* sum of all balances remain the same after proccessing transfer_from msg *)
+Lemma try_transfer_from_preserves_balances_sum : forall prev_state new_state chain ctx from to amount new_acts,
+  receive chain ctx prev_state (Some (transfer_from from to amount)) = Some (new_state, new_acts) ->
+    (sum_balances prev_state) = (sum_balances new_state).
+Proof.
+  intros * receive_some.
+  receive_simpl.
+  rename H into from_allowances.
+  rename H0 into sender_allowance.
+  rename H1 into enough_balance.
+  apply Bool.orb_false_iff in enough_balance as
+    (_ & from_enough_balance%N.ltb_ge).
+  inversion receive_some.
+  unfold sum_balances. cbn.
+  now apply sumN_FMap_add_sub.
+Qed.
+
+(* sum of all balances remain the same after approve transfer msg *)
+Lemma try_approve_preserves_balances_sum : forall prev_state new_state chain ctx delegate amount new_acts,
+  receive chain ctx prev_state (Some (approve delegate amount)) = Some (new_state, new_acts) ->
+    (sum_balances prev_state) = (sum_balances new_state).
+Proof.
+  intros * receive_some.
+  receive_simpl.
+  destruct_match in receive_some;
+    now inversion receive_some.
+Qed.
+
+
+
+(* ------------------- Contract never produces any actions ------------------- *)
+
+Lemma outgoing_acts_nil : forall (bstate : ChainState) (caddr : Address),
+  reachable bstate ->
+  env_contracts bstate caddr = Some (contract : WeakContract) ->
+  outgoing_acts bstate caddr = [].
+Proof.
+  intros * reach deployed.
+  apply (lift_outgoing_acts_nil contract); eauto.
+  intros.
+  now eapply EIP20_no_acts.
+Qed.
+
+
+
+(* ------------------- Total supply always equals inial supply ------------------- *)
+
+Lemma total_supply_eq_init_supply bstate caddr (trace : ChainTrace empty_state bstate) :
+  env_contracts bstate caddr = Some (contract : WeakContract) ->
+  exists deploy_info cstate,
+    deployment_info _ trace caddr = Some deploy_info
+    /\ contract_state bstate caddr = Some cstate
+    /\ let init_supply := init_amount deploy_info.(deployment_setup) in
+      init_supply = total_supply cstate.
+Proof.
+  apply (lift_dep_info_contract_state_prop contract); intros *.
+  - intros init_some.
+    now inversion init_some.
+  - intros IH receive_some.
+    destruct msg. destruct m.
+    + now apply try_transfer_preserves_total_supply in receive_some.
+    + now apply try_transfer_from_preserves_total_supply in receive_some.
+    + now apply try_approve_preserves_total_supply in receive_some.
+    + receive_simpl.
+Qed.
+
+
+
+(* ------------------- Sum of balances always equals total supply ------------------- *)
+
+Lemma sum_balances_eq_total_supply bstate caddr :
+  reachable bstate ->
+  env_contracts bstate caddr = Some (contract : WeakContract) ->
+  exists cstate,
+    contract_state bstate caddr = Some cstate
+    /\ (total_supply cstate) = (sum_balances cstate).
+Proof.
+  intros.
+  apply (lift_contract_state_prop contract); eauto; intros *.
+  - intros init_some.
+    inversion_clear init_some.
+    unfold sum_balances.
+    setoid_rewrite FMap.elements_add; auto.
+    setoid_rewrite FMap.elements_empty. cbn. lia.
+  - intros IH receive_some.
+    destruct msg. destruct m.
+    + now erewrite try_transfer_preserves_balances_sum,
+        try_transfer_preserves_total_supply in IH.
+    + now erewrite try_transfer_from_preserves_balances_sum,
+        try_transfer_from_preserves_total_supply in IH.
+    + now erewrite try_approve_preserves_balances_sum,
+        try_approve_preserves_total_supply in IH.
+    + receive_simpl.
+Qed.
+
+End Theories.
 End EIP20Token.
